graph.v
@@ -35,8 +35,6 @@ Module SP := FSetProperties.Properties S.
 (** And similarly for functional maps over positives *)
 
 Module M <: FMapInterface.S := PositiveMap.
-Print Module M.
-Print M.E.
 
 (* ################################################################# *)
 (** * Lemmas About Sets and Maps *)
@@ -398,6 +396,14 @@ Lemma Mremove_cardinal_less: forall A i (s: M.t A), M.In i s ->
         M.cardinal (M.remove i s) < M.cardinal s.
 Proof.
   intros A i s H.
+  rewrite WP.cardinal_fold.
+  rewrite WP.cardinal_fold.
+  apply WP.fold_rec_bis.
+  - scongruence.
+  - rewrite <- WP.cardinal_fold.
+    hauto use: WP.cardinal_Empty, neq_0_lt unfold: PositiveMap.Empty, PositiveMap.In.
+  - intros k e a m' H0 H1 H2.
+    rewrite <- WP.cardinal_fold in *.
 (** Look at the proof of [Sremove_cardinal_less], if you succeeded
    in that, for an idea of how to do this one.   *)
 
@@ -473,10 +479,9 @@ Definition no_selfloop (g: graph) := forall i, ~ S.In i (adj g i).
 
 Definition nodes (g: graph) := Mdomain g.
 
-Definition subset_nodes 
+Definition subset_nodes
                     (P: node -> nodeset -> bool)
-                    (g: graph) :=
-   M.fold (fun n adj s => if P n adj then S.add n s else s) g S.empty.
+                    (g: graph) := Mdomain (WP.filter P g).
 
 (** A node has "low degree" if the cardinality of its adjacency set is less than [K] *)
 
@@ -496,33 +501,8 @@ Lemma subset_nodes_sub:  forall P g, S.Subset (subset_nodes P g) (nodes g).
 Proof.
   intros P g.
   unfold subset_nodes.
-  apply WP.fold_rec_bis.
-  - qauto use: WP.F.In_m, Sin_domain unfold: PositiveSet.elt, PositiveSet.Subset, nodes.
-  - sfirstorder.
-  - intros k e a m' H H0 H1.
-    (* H: k maps to e in g
-       H0: k is not in m'
-       H1: a is a subset of nodes of m'
-       =============
-       want to show that (if P k e then S.add k a else a) is a subset of
-       the nodes of (M.add k e m')
-     *)
-    sdestruct (P k e).
-    + (* want to show that (S.add k a) is a subset of nodes in (M.add k e m') *)
-      unfold S.Subset in *.
-      intros a' Ha'.
-      unfold nodes.
-      apply Sin_domain.
-      destruct (E.eq_dec a' k).
-      * subst.
-        hfcrush use: WF.add_in_iff unfold: PositiveSet.elt, nodeset, PositiveMap.key.
-      * qauto use: WF.add_neq_in_iff, PositiveSet.add_3, Sin_domain unfold: nodes, PositiveSet.elt, PositiveMap.key.
-    + (* want to show that a is a subset of nodes of (M.add k e m') *)
-      unfold S.Subset in *.
-      intros a' Ha'.
-      destruct (E.eq_dec a' k).
-      * subst. qauto use: Sin_domain unfold: PositiveSet.elt, PositiveMap.key, nodes.
-      * hauto lq: on use: WF.add_in_iff, Sin_domain unfold: nodes, PositiveMap.key, PositiveSet.elt.
+  intros i Hi.
+  qauto use: WP.filter_iff, Sin_domain unfold: nodes.
 Qed.
 (** [] *)
 
@@ -533,7 +513,7 @@ Lemma select_terminates:
    M.cardinal (remove_node n g) < M.cardinal g.
 Proof.
   intros K g n H.
-  
+  unfold remove_node.
 (* FILL IN HERE *) Admitted.
 (** [] *)
 
