restrict.v
@@ -11,14 +11,13 @@ Import Arith.
 Import ListNotations.
 Import Nat.
 
-(* Restrict a map by a set of keys*)
+(* Restrict a map by a set of keys *)
 (* Fold over the set we are restricting with for better induction. *)
 Definition restrict {A} (m : M.t A) s :=
   S.fold (fun k m' => match M.find k m with
                    | Some v => M.add k v m'
                    | None => m'
                    end) s (@M.empty _).
-
   
 Lemma restrict_subset_keys {A} : forall (m : M.t A) s, S.Subset (Mdomain (restrict m s)) (Mdomain m).
 Proof.
@@ -36,6 +35,13 @@ Proof.
     + assumption.
 Qed.
 
+Lemma restrict_incl {A} :
+  forall s (f : M.t A) i, M.In i (restrict f s) -> M.In i f.
+Proof.
+  hauto lq: on use: @restrict_subset_keys, Sin_domain unfold: PositiveSet.Subset, PositiveSet.elt, PositiveMap.key.
+Qed.
+
+  
 Lemma restrict_restricts {A} :
   forall s (f : M.t A) i, S.In i s -> M.In i f -> M.In i (restrict f s).
 Proof.
@@ -78,6 +84,24 @@ Proof.
     + hauto use: PositiveMap.gso unfold: PositiveSet.elt, PositiveMap.key inv: option.
 Qed.
 
+Lemma restrict_agree_2 {A} : forall (m : M.t A) s k,
+    S.In k s -> M.find k m = M.find k (restrict m s).
+Proof.
+  intros m s k H.
+  destruct (M.find k m) eqn:E.
+  - hfcrush use: @restrict_agree, @restrict_restricts, WF.in_find_iff unfold: PositiveMap.key, PositiveSet.elt inv: option.
+  - apply not_not.
+    {
+      unfold decidable.
+      remember (M.find k (restrict m s)) as y.
+      destruct y; sfirstorder.
+    }
+    intros contra.
+    destruct (M.find k (restrict m s)) eqn:E2.
+    + qauto use: @restrict_agree unfold: PositiveSet.elt, PositiveMap.key.
+    + contradiction.
+Qed.
+
 (* Being in the restriction is enough evidence to be in the set *)
 Lemma restrict_in_set {A} : forall (m : M.t A) s k v,
     M.find k (restrict m s) = Some v ->
@@ -92,4 +116,39 @@ Proof.
     destruct (E.eq_dec k x).
     + subst. hauto l: on use: PositiveSet.add_1.
     + hauto use: PositiveSet.add_2, PositiveMap.gso unfold: PositiveMap.key, PositiveSet.elt inv: option.
+Qed.
+
+Lemma restrict_m {A} : forall s s',
+    S.Equal s s' ->
+    forall k k' : M.t A, M.Equal k k' -> M.Equal (restrict k s) (restrict k' s').
+Proof.
+  intros s s' H k k' H0.
+  unfold restrict.
+  (* Need to strengthen induction hypothesis, the maps are equal at every stage. *)
+  apply SP.fold_rec_bis.
+  - scongruence.
+  - admit.
+  - admit.
+Admitted.
+    
+
+Lemma restrict_map_comm {A B} : forall (m : M.t A) (f : A -> B) s,
+    M.Equal (M.map f (restrict m s)) (restrict (M.map f m) s).
+Proof.
+  intros m f s.
+  apply WF.Equal_mapsto_iff.
+  unfold M.MapsTo.
+  intros k e.
+  split; intros H.
+  - rewrite WF.map_o in H.
+    destruct (M.find k (restrict m s)) eqn:E; [|scongruence].
+    simpl in H.
+    rewrite <- H.
+    pose proof (restrict_in_set m s k _ E).
+    eapply restrict_agree in E.
+    pose proof (restrict_agree_2 m _ _ H0).
+    pose proof (restrict_agree_2 (M.map f m) s k H0).
+    ssimpl.
+    qauto use: WF.map_o unfold: PositiveMap.MapsTo, option_map.
+  - hfcrush use: WF.map_o, @restrict_in_set, @restrict_agree_2 unfold: PositiveSet.elt, PositiveMap.key.
 Qed.
